\documentclass{article}
\usepackage{iftex}
\usepackage{ifthen}
\usepackage{epsfig}
\usepackage[utf8]{inputenc}
\usepackage{xcolor}
% Packages requested by user
\usepackage{amsmath}
\usepackage{amssymb}

\ifPDFTeX
\usepackage{newunicodechar}
  \makeatletter
    \def\doxynewunicodechar#1#2{%
    \@tempswafalse
    \edef\nuc@tempa{\detokenize{#1}}%
    \if\relax\nuc@tempa\relax
      \nuc@emptyargerr
    \else
      \edef\@tempb{\expandafter\@car\nuc@tempa\@nil}%
      \nuc@check
      \if@tempswa
        \@namedef{u8:\nuc@tempa}{#2}%
      \fi
    \fi
  }
  \makeatother
  \doxynewunicodechar{⁻}{${}^{-}$}% Superscript minus
  \doxynewunicodechar{²}{${}^{2}$}% Superscript two
  \doxynewunicodechar{³}{${}^{3}$}% Superscript three

\fi
\pagestyle{empty}
\begin{document}
$1/(1 + \exp(-\vec{w}^T \vec{x}))$
\pagebreak

$\exp(\vec{w}^T \vec{x})$
\pagebreak

$\displaystyle P = 1 - \prod_{i=0}^{n}{\left(1 - \frac{i}{2^{64}}\right)}$
\pagebreak

$n$
\pagebreak

$\displaystyle P = 1 - \exp(\frac{-n^2}{2^{64}})$
\pagebreak

$n = 2^{28}$
\pagebreak

$0.004^N$
\pagebreak

$1.5 \times 10^{-5}$
\pagebreak

$[ i \lfloor m / \min(m,n) \rfloor, (i+1) \lfloor m / \min(m,n) \rfloor)$
\pagebreak

$m$
\pagebreak

$\displaystyle f_{a,b}(x) = ((ax + b)\ \textup{mod}\ p)\ \textup{mod}\ m$
\pagebreak

$\displaystyle f(\{x_i\}) = \sum_i{h_i(x_i)}\ \textup{mod}\ m$
\pagebreak

$h_i(.)$
\pagebreak

$2^{32}$
\pagebreak

$2^{64}$
\pagebreak

$(ax + b)\textup{ mod }p \neq ((ax + b)\textup{ mod }2^{64})\textup{ mod }p$
\pagebreak

$p = 4294967291$
\pagebreak

$p$
\pagebreak

$Z/p$
\pagebreak

$\displaystyle h_{a,b}\ :\ U \rightarrow [m-1]$
\pagebreak

$\displaystyle h_{a,b}\ :\ U \rightarrow [2^{32}]$
\pagebreak

$\displaystyle h\ :\ U \rightarrow [m-1]$
\pagebreak

$\left(\Sigma, S, \delta, s_0\right)$
\pagebreak

$\Sigma$
\pagebreak

$S$
\pagebreak

$\delta$
\pagebreak

$\delta : S \cross \Sigma \leftarrow S$
\pagebreak

$s_0$
\pagebreak

$O(N)$
\pagebreak

$N^{th}$
\pagebreak

$\delta : \Sigma \times S \rightarrow S$
\pagebreak

$\displaystyle arg\min_w{ \lambda w^2 -\sum_i{ a_i \log(S(p_i + w)) + (1 - a_i) \log(1 - S(p_i + w)) } }$
\pagebreak

$\displaystyle arg\min_w{ \lambda w^2 -\sum_{B}{ c_{1,B} \log(S(\bar{p}_B + w)) + c_{0,B} \log(1 - S(\bar{p}_B + w)) } }$
\pagebreak

$B$
\pagebreak

$\bar{p}_B$
\pagebreak

$c_{0,B}$
\pagebreak

$c_{1,B}$
\pagebreak

$\displaystyle arg\min_w{ \lambda \|w\|^2 -\sum_i{ \log([softmax(p_i + w)]_{a_i}) } }$
\pagebreak

$a_i$
\pagebreak

$\displaystyle arg\min_w{ \lambda \|w\|^2 -\sum_P{ c_{a_i, P} \log([softmax(\bar{p}_P + w)]) } }$
\pagebreak

$P$
\pagebreak

$\bar{p}_P$
\pagebreak

$c_{a_i, P}$
\pagebreak

$\{a_i\}$
\pagebreak

$(\log(1+p) - \log(1+a))^2$
\pagebreak

$p_i$
\pagebreak

$\displaystyle l_i(p) = c_i + w_i(p - a_i)^2$
\pagebreak

$w_i = \frac{\log(1+p_i) - \log(1+a_i)}{(1+p_i)(p_i-a_i)}$
\pagebreak

$c_i$
\pagebreak

$l_i(p_i) = (\log(1+p_i) - \log(1+a_i))^2$
\pagebreak

$\delta^2 (\sqrt{1 + \frac{(a - p)^2}{\delta^2}} - 1)$
\pagebreak

\[
    l_i(p) = \delta^2 \left(\sqrt{1 + \frac{(a_i - p_i)^{2}}{\delta^2}} - 1\right) +
             \frac{-a_i+p_i}{\sqrt{\frac{\delta^2 + (a_i-p_i)^{2}}{\delta^2}}} (p - p_i) +
             \frac{-a_i+p_i}{2\sqrt{\frac{\delta^2 + (a_i-p_i)^{2}}{\delta^2}}(a_i-p_i)} (p - p_i)^2
\]
\pagebreak

$p = p_i$
\pagebreak

\[\frac{-a_i + p_i}{\sqrt{\frac{\delta^2 + (a_i - p_i)^2}{\delta^2}}}\]
\pagebreak

\[\frac{1}{\sqrt{1 + \frac{(a_i - p_i)^2}{\delta^2}}}\]
\pagebreak

$\displaystyle l_i(p) = -(1 - a_i) \log(1 - S(p)) - a_i \log(S(p))$
\pagebreak

$S(\cdot)$
\pagebreak

$\displaystyle l_i(p) = -\sum_i a_{ij} \log(\sigma(p))$
\pagebreak

$\sigma(p)$
\pagebreak

$[\sigma(p)]_j = \frac{e^{p_i}}{\sum_k e^{p_k}}$
\pagebreak

$x^* = arg\min_x\{\sum_i{L(p_i + x, a_i)}\}$
\pagebreak

$n_A$
\pagebreak

$n_B$
\pagebreak

$k$
\pagebreak

$\frac{n_A}{k}$
\pagebreak

$\frac{n_B}{k}$
\pagebreak

$\sum_{x,y} P(x,y) \log\left(\frac{P(x,y)}{P(x)P(y)}\right)$
\pagebreak

$k l < B(n)$
\pagebreak

$l$
\pagebreak

$B(n) = n^{\alpha}$
\pagebreak

$\alpha < 1$
\pagebreak

$O(N^2)$
\pagebreak

$A = \{x_i\}$
\pagebreak

$B = \{x_j\}$
\pagebreak

$\displaystyle d_s(A, B) = min_{i,j}{d(x_i, x_j)$
\pagebreak

$\displaystyle d_c(A,B) = min_{i,j}{d(x_i, x_j)$
\pagebreak

$M(n, N) = \sum_{i=1}^{N}{ (x_i - M(1, N))^n } = \sum_{i=1}^{N}{ (x_i - M(1, N-1) + (M(1, N-1) - M(1, N)))^n }$
\pagebreak

$M(1, N)$
\pagebreak

$N$
\pagebreak

$n > 1$
\pagebreak

$O(N log(n))$
\pagebreak

$n << N$
\pagebreak

$(x, f(x), \sigma^2(x))$
\pagebreak

$\sigma^2(x)$
\pagebreak

$f(x)$
\pagebreak

$\displaystyle arg\max_x \doubleE_x[max(f^* - f, 0)]$
\pagebreak

$\displaystyle K(x,y|\theta_0, \theta_1) = \theta_0^2 exp(-(x-y)^t D(\theta_1) (x-y)))$
\pagebreak

$[D(\theta_1)]_{ij} = (\theta_{1,i}^2 + \epsilon)\delta_{ij}$
\pagebreak

$\epsilon$
\pagebreak

$\displaystyle P\left(\left|\frac{e}{n} - 1\right| > \epsilon\right) < \delta$
\pagebreak

$e$
\pagebreak

$\displaystyle O\left(\left|\frac{1}{\epsilon^2}\log(\epsilon)log(\delta)\right|\right)$
\pagebreak

$\displaystyle (44 + 3m)k$
\pagebreak

$m = 1/\epsilon^2$
\pagebreak

$k = -\log(\delta)$
\pagebreak

$O(m)$
\pagebreak

$A^{(i)}$
\pagebreak

$B^{(j)}$
\pagebreak

$\Omega_i$
\pagebreak

$\Omega_j$
\pagebreak

$\displaystyle \frac{\| A^{(i)} \cap B^{(j)} \|}{ \| \Omega_i \cup B^{(j)} \| }$
\pagebreak

$\displaystyle \frac{\| A^{(i)} \cap B^{(j)} \|}{ \| A^{(i)} \cup \Omega_j \| }$
\pagebreak

$|A|$
\pagebreak

$V - |A|$
\pagebreak

$\(\{n_i\}\)$
\pagebreak

$\(\displaystyle f(\{n_j\}) = \frac{n!}{\prod_i{n_j}}\prod_i{p_j^{n_j}}\)$
\pagebreak

$\(n = \sum_i{n_i}\)$
\pagebreak

$\(\displaystyle \sum_{\{n_j : f(\{n_j\}) \leq f(\{n_i\})\} }{ f(\{n_j\}) }\)$
\pagebreak

$\displaystyle \sum_{\{\{n_j\}:\sum{n_j}=n\}} H(n_k) n! \prod_{j=1}^m\frac{p_j^{n_j}}{n_j!}$
\pagebreak

$H(.)$
\pagebreak

$\displaystyle E[unique(Y)]=\sum_{\{\{n_j\}:n_j>0,\sum{n_j}=n\}}kn!\prod_{j=1}^k{\frac{p_j^{n_j}}{n_j!}} $
\pagebreak

$Y$
\pagebreak

$\binom{n}{m}$
\pagebreak

$\(\displaystyle \log\left(\frac{n!}{m!(n-m)!}p^m(1-p)^{n-m}\right)\)$
\pagebreak

$\(m \leq n\)$
\pagebreak

$\(\displaystyle \log\left(\frac{n!}{ \prod_i{n_i!} }p^n_i\right)\)$
\pagebreak

$\(n = sum_i{n_i}\)$
\pagebreak

$f(x) = x - c$
\pagebreak

$f(x) = -x$
\pagebreak

$f(x) = e^x$
\pagebreak

$h(x) = f(x)g(x)$
\pagebreak

$x - c$
\pagebreak

$(\epsilon, \rho)$
\pagebreak

$-p_i \log(p_i)$
\pagebreak

$T$
\pagebreak

$k = O\left(\frac{1}{\epsilon^2}\right)$
\pagebreak

$\frac{1}{\epsilon^2} \log(T) \log(\frac{T}{\epsilon}$
\pagebreak

$Y - u$
\pagebreak

$u$
\pagebreak

$a$
\pagebreak

$b$
\pagebreak

$P([a,m]) = P([m,b]) = p / 100 / 2$
\pagebreak

$\displaystyle mean = \frac{a}{b}$
\pagebreak

$\displaystyle variance = \frac{a}{b^2}$
\pagebreak

$\displaystyle a_i' = \frac{a}{\gamma_i}$
\pagebreak

$\displaystyle b_i' = \frac{b}{\gamma_i}$
\pagebreak

$\displaystyle f(x_i) = \frac{(b_i')^{a_i'}}{\Gamma(a_i')}x_i^{a_i'-1}e^{-b_i'x_i}$
\pagebreak

$-\log(\prod_i{F(x_i)})$
\pagebreak

$F(.)$
\pagebreak

$\{x_i\}$
\pagebreak

$\gamma_i$
\pagebreak

$(0,\infty)$
\pagebreak

$X = Y - u$
\pagebreak

$-u$
\pagebreak

$BIC = -2 log(L(x)) - k log(n)$
\pagebreak

$L(x)$
\pagebreak

$AIC_c = -2 log(L(x)) + 2 k + \frac{k(k+1)}{n - k - 1}$
\pagebreak

$m = \frac{1}{n}\sum_{i=1}{n}{x_i}$
\pagebreak

$v = \sum_{i=1}{n}{ (x_i - m)^t (x_i - m) }$
\pagebreak

$frac{D(D+1)}{2}$
\pagebreak

$p = \left \lceil \log_2(x) \right \rceil$
\pagebreak

$\frac{n!}{k!(n-k)!}$
\pagebreak

$O(2^l l^d)$
\pagebreak

$2^l$
\pagebreak

$d$
\pagebreak

$O(2^{ld}$
\pagebreak

$\|I\|_1 = l$
\pagebreak

$I$
\pagebreak

$\sqrt{\sum_i x_i^2}$
\pagebreak

$O(k)$
\pagebreak

$M$
\pagebreak

$O(N + M)$
\pagebreak

$\{ \frac{x_i - m_x}{\sigma_x} \}$
\pagebreak

$P : \Omega \rightarrow \{-1, 1}$
\pagebreak

$\left( \sum_{i=1}{n}{ P_i \frac{x_i - m_x}{\sigma_x} - \sum_{i=1}{n}{ P_i \frac{y_i - m_y}{\sigma_y} \right)$
\pagebreak

$2 (1 - cov(X,Y))$
\pagebreak

$cov(X,Y)$
\pagebreak

$X$
\pagebreak

$\frac{1}{n}\sum_{i=1}{n}{\frac{(x-m_x)(y-m_y)}{\sigma_x\sigma_y}}$
\pagebreak

$|f(x_k) - f(x_{k-1})| < \epsilon |f(x_k) - f(x_0)|$
\pagebreak

$\{(x_i, y_i)\}$
\pagebreak

$y = c_0 + c_1 x + ... + c_N x^N$
\pagebreak

$\theta^*$
\pagebreak

$\theta^* = arg\min_{\theta}{(y - X\theta)^tDiag(w)(y - X\theta)}$
\pagebreak

$[X]_{ij} = x_i^{j-1}$
\pagebreak

$2N-1$
\pagebreak

$X^tDiag(w)X$
\pagebreak

$X^tDiag(w)y$
\pagebreak

$3(N+1)$
\pagebreak

$12(N+1)$
\pagebreak

$x_i$
\pagebreak

$(x, y(x))$
\pagebreak

$x \mapsto x - b$
\pagebreak

$x$
\pagebreak

$y_i = \sum_{j=0}{N} c_j x_i^j + Y_i$
\pagebreak

$Y_i$
\pagebreak

$N(0, \sigma)$
\pagebreak

$C = (X^t X)^{-1}X^t E[YY^t] X (X^t X)^{-1}$
\pagebreak

$E[YY^t] = \sigma^2 I$
\pagebreak

$C = \sigma^2 (X^t X)^{-1}$
\pagebreak

$x^tC^{-1}x$
\pagebreak

$e^Y - u$
\pagebreak

$\displaystyle e^{m + 1/2p}$
\pagebreak

$\displaystyle (e^{1/p} - 1)e^{2m + 1/p}$
\pagebreak

$\displaystyle e^{m_i' + 1/2p_i'} = e^{m + 1/2p}$
\pagebreak

$\displaystyle (e^{1/p_i'} - 1)e^{2m_i' + 1/p_i'} = \gamma_i(e^{1/p} - 1)e^{2m + 1/p}$
\pagebreak

$m_i'$
\pagebreak

$p_i'$
\pagebreak

$\displaystyle m_i' = m + \frac{1/p - \log(1 + \gamma_i(e^{1/p} - 1))}{2}$
\pagebreak

$\displaystyle p_i' = \frac{1}{\log(1 + \gamma_i(e^{1/p} - 1))}$
\pagebreak

$\displaystyle f(x_i) = \sqrt{\frac{p_i'}{2\pi}}e^{-p_i'/2(\log(x_i) - m_i')^2}$
\pagebreak

$e ^{m + 1 / 2 p}$
\pagebreak

$\displaystyle \frac{e ^{-2m - 1 / p}}{e ^{1 / p} - 1}$
\pagebreak

$e^{m + 1 / 2 p}$
\pagebreak

$X = e^Y - u$
\pagebreak

$X = exp(s * Y + m)$
\pagebreak

$min_{a,b}\{P([a,m]) + P([m,b])\} = p / 100$
\pagebreak

$P_i = P(\{c : L(c) <= L(c_i)\})$
\pagebreak

$\displaystyle f(p_i) = \frac{\Gamma(a_0)}{\Gamma(a_0 - a_i)\Gamma(a_i)}(1 - p_i)^{a_0-a_i-1}p_i^{a_i-1}$
\pagebreak

$\displaystyle a_0 = \sum_i{a_i}$
\pagebreak

$int_{\theta}f(x|\theta, M)f(\theta|M)\d\theta$
\pagebreak

$(x,l)$
\pagebreak

$\displaystyle I=argmin{\sum_{(i,j)\in J}\sum_{k=i}^{k<j}{(x_k-\mu_{i,j})^2}}$
\pagebreak

$\mu_{i,j}=1/(j-i)\sum_{k\in[i,j)}{x_k}$
\pagebreak

$\displaystyle {(\sum_{k=i}^{k<j}{(x_k-\mu_{i,j})^2})^{1/p}}$
\pagebreak

$p\rightarrow\infty$
\pagebreak

$p = 2$
\pagebreak

$m \leq n$
\pagebreak

$O(N^2n)$
\pagebreak

$\displaystyle f(x_i) = \sqrt{\frac{p}{2\pi\gamma_i}} e^{-\frac{p}{2\gamma_i}(x_i - m)^2}$
\pagebreak

$2^{128}-1$
\pagebreak

$2^{1024}-1$
\pagebreak

$2^{512}$
\pagebreak

$[N] = {1,...,N}$
\pagebreak

$\displaystyle O(\frac{log(N)}{k})$
\pagebreak

$\displaystyle \epsilon = \frac{|r - qn|}{n}$
\pagebreak

$qn$
\pagebreak

$\displaystyle x \rightarrow \left \lfloor xn \right \rfloor$
\pagebreak

$\displaystyle q \rightarrow \frac{x}{n} + 0.5$
\pagebreak

$3k$
\pagebreak

$\sup_y{\{y:F(y)<f\}}$
\pagebreak

$[x]_i ~ N(0,1)$
\pagebreak

$\displaystyle P(x) \propto \mathbb{E}\left[ \|x - Y\|_2 \right]$
\pagebreak

$\chi^2$
\pagebreak

$\(\displaystyle f(\{n_i\}) = \frac{n!}{\prod_i{n_i}}\prod_i{p_i^{n_i}}\)$
\pagebreak

$\{n(i)\}$
\pagebreak

$\displaystyle n_i \in \{0,1,...,n\}\ \ \forall i$
\pagebreak

$\displaystyle \sum_i{n_i} = [n \sum_i{w(i)}]$
\pagebreak

$\displaystyle \sum_i{|n_i - n w(i)|}\ is\ minimized$
\pagebreak

$\frac{|A\cap B|}{|A\cup B|}$
\pagebreak

$\frac{|A\cap B|}{\min(|A|,|B|)}$
\pagebreak

$L^-_{fc}(f) = {x : f(x) <= fc}$
\pagebreak

$y_i(x) = a_i(x-x_i)^3 + b_i(x-x_i)^2 + c_i(x-x_i) + d_i$
\pagebreak

$Ax = y$
\pagebreak

$A$
\pagebreak

$c$
\pagebreak

$y$
\pagebreak

$\displaystyle \left(A + \begin{bmatrix} 1\\ 0\\ 0\\ \cdot\\u \end{bmatrix} \begin{bmatrix} 1 & 0 & 0 & \cdot & v \end{bmatrix}\right)x=y$
\pagebreak

$\frac{1}{|b-a|}\int_{[a,b]}{\left|\frac{df(s)}{ds}\right|}ds$
\pagebreak

$\displaystyle T = n\omega^2 = \frac{1}{12n}+\sum_{i=1}^n{\frac{2i-1}{2n}-F(x_{(i)})}$
\pagebreak

$x_{(i)}$
\pagebreak

$\{y\ |\ y \leq x\}$
\pagebreak

$\{y\ |\ f(y) \leq f(x)\}$
\pagebreak

$f(.)$
\pagebreak

$\{y\ |\ y \geq x\}$
\pagebreak

$E[ X 1{[a,b]} ] / E[ 1{a,b]} ]$
\pagebreak

$P(R)$
\pagebreak

$ R = \{y\ |\ f(y) \leq f(x)\} $
\pagebreak

$P(R) \rightarrow 0$
\pagebreak

$ -E[\log(f(x))] $
\pagebreak

$x^2$
\pagebreak

$sigmoid\left(\frac{sign (x - x0)}{width}\right)$
\pagebreak

$[\sigma(z)]_i = \frac{exp(z_i)}{\sum_j exp(z_j)}$
\pagebreak

$(1 - x) ^ p$
\pagebreak

$1 - (1 - x) ^ p$
\pagebreak

$\log(1 - x)$
\pagebreak

$P(\{s : f(s) < f(x)\}) = \int{I(f(s) < f(x)) f(s)}ds$
\pagebreak

$\displaystyle I(f(s) < f(x)) \approx (1+e^{-k}) \frac{e^{-k(f(s)/f(x)-1)}}{1+e^{-k(f(s)/f(x)-1)}}$
\pagebreak

$k'(s) = k(s)/f(x)$
\pagebreak

$\{y : f(y) <= f(x)\}$
\pagebreak

$Y = m + \sqrt{\lambda}(X - m)$
\pagebreak

$P(\{(s_1, ..., s_n)\ |\ L(s_1, ..., s_n) \leq \prod_{i}\frac{P_i}{2}\})$
\pagebreak

$P(i)$
\pagebreak

$ p = P(\{s\ |\ L(s) \leq L(x)\}) $
\pagebreak

$s$
\pagebreak

$ L'(s) = \frac{N!}{1!(N - 1)!} (F(s) - F(-s)) ^{(N-1)} f(s) $
\pagebreak

$ R' = \{s\ |\ L'(s) \leq L'(x)\} $
\pagebreak

$ R = \{s\ |\ s > x\ or\ s < x\} $
\pagebreak

$(-\infty, x] \bigcup [x, \infty)$
\pagebreak

$ P(R) = \frac{2N}{2N} \left[(2t - 1) ^{N}\right]_{F(x)}^1 = 1 - (1 - p) ^{N} $
\pagebreak

$(1 - F(x)) = p / 2$
\pagebreak

$x_2$
\pagebreak

$x_1$
\pagebreak

$ p_2 = P(\{s\ |\ L(s) \leq L(x_2)\}) < p_1 = P(\{s\ |\ L(s) \leq L(x_1)\}) $
\pagebreak

$(s_1, s_2, ..., s_M)$
\pagebreak

$ L'(s_1, ..., s_M) = \frac{N!}{(N-M)!} (F(s_1) - F(-s_1)) ^{N-M} \prod_{i=1}^M f(s_i) $
\pagebreak

$p_1 > p_2 > ...> p_M$
\pagebreak

$ R'' = \{s\ |\ L'(s) \leq L'(x)\} $
\pagebreak

$ R' = \{s\ |\ s_i > x_i\ or\ s_i < x_i\} $
\pagebreak

$ P(R') = 2 ^{M} P(\{s\ |\ s_i > x_i\}) $
\pagebreak

$s_i$
\pagebreak

$s_i < s_{i+1}$
\pagebreak

$i < M$
\pagebreak

$s_M < \infty$
\pagebreak

$M^2$
\pagebreak

$\{p_1, ..., p_M\}$
\pagebreak

$(x_i, y_i)$
\pagebreak

$\{(x_i, y_i = y(x_i) + Y_i\}$
\pagebreak

$\displaystyle \max_i\left\{ \int_{[a_i,b_i]}{ \left| y(x) - \left<y\right>_{[a_i,b_i]} \right| }dx \right\} $
\pagebreak

$\left<y\right>_{[a_i,b_i]} = \frac{1}{b_i-a_i}\int_{[a_i,b_i]}{y(x)}dx$
\pagebreak

$\left<y\right>$
\pagebreak

$([a_i,b_i], m_i)$
\pagebreak

$m_i$
\pagebreak

$([a+(i-1)l,b+il])$
\pagebreak

$i\in[n]$
\pagebreak

$l=(b-a)/n$
\pagebreak

$(t, f(t))$
\pagebreak

$n_i + epsilon n$
\pagebreak

$n_i$
\pagebreak

$P(1-\delta)$
\pagebreak

$([a_i,b_i], S_i)$
\pagebreak

$S_i$
\pagebreak

$([a_i,b_i])$
\pagebreak

$\(\frac{1}{(n-k)\sigma^2}\sum_{k=1}^{n-k}{(f(k) - \mu)(f(k+p) - \mu)}\)$
\pagebreak

$ \sum_i 1\{t_i \leq t < t_{i+1}\} s_i f_p(t) $
\pagebreak

$\{s_i\}$
\pagebreak

$f_p(\cdot)$
\pagebreak

$f_q(s)$
\pagebreak

$a = \max\{x \le f_q(s)\}$
\pagebreak

$b = \min{x \ge f_q(s)}$
\pagebreak

$\displaystyle \bar{s} = \frac{(y(b) - y(a))(f_q(s) - a)}{b - a}$
\pagebreak

$y(.)$
\pagebreak

$ pid \leftarrow c$
\pagebreak

$pid$
\pagebreak

$|P(b) - P(a)| < threshold \times min(P(A), P(b))$
\pagebreak

$P_{A \ B} = 1.0 - F(g(A \ B))$
\pagebreak

$g(\cdot)$
\pagebreak

$F(\cdot)$
\pagebreak

$P_{A \ B} >> P_A$
\pagebreak

$\displaystyle \left(1.0 - \frac{\log(P_{A \ B})}{\log(P_A)}\right)_0^1$
\pagebreak

$(\cdot)_0^1$
\pagebreak

$[0,1]$
\pagebreak

$\displaystyle P_{A \cap B} = \min\left\{ F(g(A \cap B)), 1-F(g(A \cap B)) \right\}$
\pagebreak

$P_{A \cap B} \lte P_A$
\pagebreak

$\displaystyle \left(\frac{\log(P_{A \cap B})}{\log(P_A)}\right)_0^1$
\pagebreak

$arg\max_S \frac{1}{|S|} \sum_{f\in S}{MIC(f,t)} - \frac{1}{|S|^2} \sum_{f\in S, g\in S} {MIC(f,g)}$
\pagebreak

$(x_i, \gamma_i)$
\pagebreak

$i^{th}$
\pagebreak

$10^8$
\pagebreak

$10^{-8}$
\pagebreak

$\displaystyle \max_{a \in A, b \in B}{d[a,b]}$
\pagebreak

$\displaystyle \frac{1}{|A||B|}\sum_{a \in A, b \in B}{d[a,b]}$
\pagebreak

$\(\displaystyle e^{m+\frac{1}{p}\left(\frac{1}{t} + 1\right)} f(p)\)$
\pagebreak

$sum_i{(\log(x_i) - \frac{1}{n}sum_j{\log(x_j)})^2}$
\pagebreak

$\displaystyle \int{L(x_i\ |\ p)f(p)}dp = \Gamma(\sum_j{a_j})\int_{p\in S}{p_i\prod_j{\frac {p_j^{a_j-1}}{\Gamma(a_j)}}}dp_j $
\pagebreak

$\displaystyle R = \{p\ |\ \left\|p\right\|_1 = 1\}$
\pagebreak

$\displaystyle \frac{\Gamma(a_0)\Gamma(a_i + 1)}{\Gamma(a_0 + 1)\Gamma(a_i)} = \frac{a_i}{a_0}$
\pagebreak

$\displaystyle F(x) = \frac{1}{a_0}\sum_{\{i : x_i \leq x\}}{a_i}$
\pagebreak

$\displaystyle F^c(x) = \frac{1}{a_0}\sum_{\{i : x_i \geq x\}}{a_i}$
\pagebreak

$F^c(x) \neq 1 - F(x)$
\pagebreak

${x_i}$
\pagebreak

$\alpha$
\pagebreak

$\beta$
\pagebreak

$\displaystyle \frac{1}{B(\alpha,\beta)}x^{\alpha-1}(1-x)^{beta-1}$
\pagebreak

$P(D > observed) = Q_{KS}\left(\left(\sqrt{N_e}+0.12+\frac{0.11}{\sqrt{N_e}}\right) D\right)$
\pagebreak

$Q_{KS}(\lambda)=2\sum_{j=1}^{\infty}{(-1)^{j-1}e^{-2j^2\lambda^2}}$
\pagebreak

$\max(-2\log(L(\{x_i\}|M_1)) + 2\log(L(\{x_i\}|M_2)) + (n_1 - n_2) \log(n), 0)$
\pagebreak

$M_1$
\pagebreak

$M_2$
\pagebreak

$n_1$
\pagebreak

$n_2$
\pagebreak

$m_{a,b} = a F(a) + \int_a^b{x f(x)}dx + b (1 - F(b))$
\pagebreak

$m_{a,b} = (a-m_{a,b})^2 F(a) + \int_a^b{(x-m_{a,b})^2 f(x)}dx + (b-m_{a,b})^2 (1 - F(b))$
\pagebreak

$x(i)$
\pagebreak

$P(R(i))$
\pagebreak

$z(i)$
\pagebreak

$\displaystyle \frac{1 + erf(-z(i))}{2} = \frac{P(R(i))}{2}$
\pagebreak

$\displaystyle \{P_i\ :\ i = 1, ..., m \}$
\pagebreak

$\displaystyle P_m < P_{m-1} < ... < P_1$
\pagebreak

$\displaystyle \frac{N!}{(N-m)!}\int_{0}^{P_m}\int_{t_m}^{P_{m-1}}...\int_{t_2}^{P_1}(1-t_1)^{N-m}dt_1...dt_m$
\pagebreak

$t_i$
\pagebreak

\end{document}
